-worked on LM->TM NP reduction

theories/L/Complexity/Reductions/TMGenNP/M_LM2TM.v
@@ -1,22 +1,165 @@
 From Undecidability.L.Complexity Require Import NP.
-From Undecidability.TM Require TM ProgrammingTools CaseList.
+From Undecidability.TM Require TM ProgrammingTools CaseList CaseBool Code.Decode Code.DecodeList.
 From Undecidability.TM Require Import TM SizeBounds.
 
-From Undecidability.L.Complexity  Require Import TMGenNP_fixed_mTM.
+From Undecidability.L.Complexity  Require Import TMGenNP_fixed_mTM UpToCNary.
 
-From Undecidability.LAM Require HaltingProblem.
 From Undecidability.L.AbstractMachines Require Import FlatPro.Programs.
      
 Unset Printing Coercions.
-From Coq.ssr Require ssrfun.
-Module Option := ssrfun.Option.
+
+From Undecidability.LAM Require Alphabets.
 
 From Coq Require Import Lia Ring Arith.
 
 From Undecidability.L.Complexity  Require Import GenNP_is_hard LMGenNP TMGenNP_fixed_mTM.
 Check fun M =>
-  restrictBy (LMHaltsOrDiverges Pro) (LMGenNP Pro) ⪯p (restrictBy (HaltsOrDiverges_fixed_mTM M) (TMGenNP_fixed_mTM M)).
+  restrictBy (LMHaltsOrDiverges _) (LMGenNP (list bool)) ⪯p (restrictBy (HaltsOrDiverges_fixed_mTM M) (TMGenNP_fixed_mTM M)).
 
+From Undecidability Require Import Code.ListTM_concat_repeat.
+
+Module BoollistToEnc.
+
+
+  Definition enc_bool_perElem (b:bool) := [lamT;lamT;varT 0;lamT; lamT; varT (if b then 1 else 0); retT; retT;appT].
+  Definition enc_bool_nil := [lamT; lamT; varT 1; retT; retT].
+  Definition enc_bool_closing :=  [appT; retT; retT].
+
+  Lemma enc_bool_explicit (bs : list bool):
+    compile (Computable.enc bs) = flat_map enc_bool_perElem bs ++ enc_bool_nil ++ concat (repeat enc_bool_closing (length bs)).
+  Proof.
+    unfold Computable.enc. cbn. unfold Lists.list_enc. cbn. unfold LBool.bool_enc.
+    induction bs as [ | b bs]. reflexivity.
+    cbn - [concat repeat]. rewrite IHbs. replace (S (| bs |)) with (|bs|+1) by nia.
+    destruct b;cbn - [concat repeat]. all:repeat (autorewrite with list; cbn - [concat repeat]). all:repeat f_equal.
+    all:rewrite repeat_add_app,concat_app. all:easy.
+  Qed.
+
+  Arguments enc_bool_perElem : simpl never.
+  
+  Section M.
+    Import ProgrammingTools Combinators ListTM CaseList CaseBool.
+    Import Alphabets.
+
+
+    Variable (sig : finType).
+    (* Hypothesis (defX: inhabitedC sigX). *)
+
+    (* We use the FinType instance of bool, as it has a Case-machine *)
+    
+    Context `{retr__list : Retract (sigList bool) sig}
+            `{retr__Pro : Retract Alphabets.sigPro sig}
+            `{retr__nat : Retract sigNat sig}.
+    Local Instance retr__bool : Retract bool sig := ComposeRetract retr__list (Retract_sigList_X _).
+  
+    Check _ : codable sig (list bool).
+    Check _ : codable sig bool.
+
+    (* Tapes: 
+       0: bs (input)
+       1: result 
+       2: intern (constant for ConcatRepeat [0])
+       3: intern (length of bs for concatReepat [1])
+     *)
+    
+    Definition Rel : pRel sig^+ unit 4 :=
+      ignoreParam
+        (fun tin 'tout =>
+           forall (bs : list bool),
+             tin[@Fin0] ≃ bs 
+             -> isRight tin[@Fin1]
+             -> isRight tin[@Fin2]
+             -> isRight tin[@Fin3]
+             -> isRight tout[@Fin0]
+               /\ tout[@Fin1]  ≃ compile (Computable.enc (rev bs))
+               /\ isRight tin[@Fin2]
+               /\ isRight tin[@Fin3]).
+
+    (* für step (prepend the bs-dependent symbols) 
+               Tapes: 
+       0: bs (input)
+       1: result 
+       2: head of bs
+       3: intern (length of bs for concatReepat [1])
+     *)
+
+    Definition M__step : pTM sig^+ (option unit) 4 :=
+      If (LiftTapes (ChangeAlphabet (CaseList.CaseList _) retr__list) [|Fin0;Fin2|])
+         (Switch (LiftTapes (ChangeAlphabet CaseBool retr__bool) [|Fin2|])
+                 (fun b => LiftTapes (ChangeAlphabet (WriteValue (encode (enc_bool_perElem b))) _) [| Fin2|];;
+                        LiftTapes (ChangeAlphabet (App' _) _) [|Fin2;Fin1|];;
+                        Return (LiftTapes (Reset _) [|Fin2|]) None))
+         (Return (LiftTapes (Reset _) [|Fin0|]) (Some tt)).
+
+    Definition Rel__step : pRel sig^+ (option unit) 4 :=
+      (fun tin '(yout,tout) =>
+           forall (bs : list bool) (res : Pro),
+             tin[@Fin0] ≃ bs 
+             -> tin[@Fin1] ≃ res
+             -> isRight tin[@Fin2]
+             -> match bs,yout with
+                 [],  Some _ => isRight tout[@Fin0] /\ tout[@Fin1] = tin[@Fin1]
+               | (b::bs),None => tout[@Fin0] ≃ bs /\ tout[@Fin1] ≃ enc_bool_perElem b++res
+               | _,_ => False
+               end
+               /\ isRight tin[@Fin2]
+               /\ tout[@Fin3] = tin[@Fin3]).
+
+    
+    Lemma Realises__step : M__step ⊨ Rel__step .
+    Proof.
+      eapply Realise_monotone.
+      {unfold M__step. TM_Correct_noSwitchAuto. TM_Correct.
+       2,3: now (notypeclasses refine (@Reset_Realise _ _ _ _ _);shelve).
+       intros b. TM_Correct. 2:now (notypeclasses refine (@Reset_Realise _ _ _ _ _);shelve).
+       now apply App'_Realise. }
+      intros t (y,t') H. cbn. 
+      intros bs res Hbs Hres Ht2. 
+      destruct H as [H|H].
+      -cbn in H. TMSimp. modpon H;[]. destruct bs. now exfalso.
+       TMSimp. modpon H0;[]. modpon H1;[]. modpon H2;[]. TMSimp.
+       repeat (simple apply conj). all:try contains_ext. now isRight_mono. reflexivity. 
+      -cbn in H. TMSimp. modpon H;[]. destruct bs. 2:easy. TMSimp.
+       modpon H1;[]. modpon H0; [].
+       repeat (simple apply conj). all:try now isRight_mono. all:reflexivity.
+       Unshelve. 4:eauto. 2:easy.
+    Qed.
+
+    Definition M__loop : pTM sig^+ unit 4 := While M__step.
+
+    
+
+    Definition M : pTM sig^+ unit 4 :=
+      LiftTapes (Length retr__list retr__nat) [|Fin0;Fin1;Fin2;Fin3|];;
+      LiftTapes (ChangeAlphabet (WriteValue (encode (enc_bool_closing))) _) [|Fin2|];;
+      LiftTapes (ConcatRepeat.M retr__list retr__nat) [|Fin2;Fin3;Fin1|];;
+      LiftTapes (Reset _) [|Fin2|];;
+      LiftTapes (ChangeAlphabet (WriteValue (encode  (enc_bool_nil))) _ ) [|Fin2|];;
+      LiftTapes (ChangeAlphabet (App' _) _) [|Fin2;Fin1|];;
+      M__loop.
+
+
+    (*
+    Context (sig F:finType) (n:nat) (M__multi : pTM sig F n).
+
+      (*TODO: Check that tape contaisn Encoding of programm*)
+  (*
+      Definition M : pTM _ _ 12 := LiftTapes HaltingProblem.Loop [|Fin1,Fin2,|].
+
+      Definition Rel : pRel ((sigList (sigTape sig)) ^+) (option F) 1 :=
+        fun t '(y,t') => match y with
+                        None => ~ exists (v : tapes sig n), StepTM.contains_tapes t[@Fin0] v
+                      | Some y => exists (v v': tapes sig n), StepTM.contains_tapes t[@Fin0] v
+                                                        /\ StepTM.contains_tapes t'[@Fin0] v'
+                                                        /\ Canonical_Rel M__multi v (y,v')
+                      end.
+  *) *)
+  End M.
+End BoollistToEnc.
+
+From Undecidability.LAM Require HaltingProblem.
+
+  
 Module LMtoTM.
   Module LAM := LAM.TM.HaltingProblem.
   Section sec.
